step pred from trace coh

src/reordering/Reordering.v
@@ -1,20 +1,13 @@
-Require Import Core.
+Require Import AuxDef Core Lia.
 Require Import ReordSimrel ReorderingMapper.
 Require Import ReorderingExecA ReorderingExecB.
 Require Import ReordExecNaNb ReorderingReexec.
+Require Import ThreadTrace TraceSwap.
 
 From hahn Require Import Hahn.
 From hahnExt Require Import HahnExt.
 From imm Require Import Events Execution.
 Require Import Setoid Morphisms Program.Basics.
-
-Section ReorderingSteps.
-
-Variable X_t X_t' X_s : WCore.t.
-Variable a_t b_t : actid.
-Variable traces_t traces_s : thread_id -> trace label -> Prop.
-
-Notation "'mapper'" := (mapper a_t b_t).
 
 Definition event_mem (a : actid) (t : trace label) : Prop :=
   match t, a with
@@ -22,6 +15,67 @@ Definition event_mem (a : actid) (t : trace label) : Prop :=
   | trace_inf _, _ => True
   | trace_fin l, ThreadEvent _ n => n < length l
   end.
+
+Lemma event_memE G e
+    (NINIT : tid e <> tid_init)
+    (CONT : contigious_actids G) :
+  event_mem e (thread_trace G (tid e)) <->
+    acts_set G e.
+Proof using.
+  destruct e as [el | et en]; ins.
+  red in CONT. destruct (CONT _ NINIT) as [N EQ].
+  split; intros HSET.
+  { enough (IN' :
+      (acts_set G ∩₁ (fun e => et = tid e))
+        (ThreadEvent et en)
+    ).
+    { apply IN'. }
+    apply EQ, thread_set_iff.
+    unfold thread_trace, thread_actid_trace in HSET.
+    ins. rewrite EQ, thread_seq_set_size in HSET.
+    ins. now autorewrite with calc_length in HSET. }
+  unfold thread_trace, thread_actid_trace.
+  ins. rewrite EQ, thread_seq_set_size.
+  ins. autorewrite with calc_length.
+  eapply thread_set_iff, EQ. basic_solver.
+Qed.
+
+Section ReorderingSteps.
+
+Variable X_t X_t' X_s : WCore.t.
+Variable rtid : thread_id.
+Variable i_b : nat.
+Variable traces_t traces_s : trace_storage.
+
+Definition i_a := i_b + 1.
+
+Notation "'G_t'" := (WCore.G X_t).
+Notation "'lab_t'" := (lab G_t).
+Notation "'loc_t'" := (loc lab_t).
+Notation "'val_t'" := (val lab_t).
+Notation "'E_t'" := (acts_set G_t).
+Notation "'sb_t'" := (sb G_t).
+Notation "'rf_t'" := (rf G_t).
+Notation "'co_t'" := (co G_t).
+Notation "'rmw_dep_t'" := (rmw_dep G_t).
+Notation "'data_t'" := (data G_t).
+Notation "'ctrl_t'" := (ctrl G_t).
+Notation "'addr_t'" := (addr G_t).
+Notation "'W_t'" := (fun e => is_true (is_w lab_t e)).
+Notation "'R_t'" := (fun e => is_true (is_r lab_t e)).
+Notation "'F_t'" := (fun e => is_true (is_f lab_t e)).
+Notation "'Loc_t_' l" := (fun e => loc_t e = l) (at level 1).
+Notation "'Val_t_' l" := (fun e => val_t e = l) (at level 1).
+Notation "'same_loc_t'" := (same_loc lab_t).
+Notation "'same_val_t'" := (same_val lab_t).
+Notation "'Acq_t'" := (fun e => is_true (is_acq lab_t e)).
+Notation "'Rel_t'" := (fun e => is_true (is_rel lab_t e)).
+Notation "'Rlx_t'" := (fun e => is_true (is_rlx lab_t e)).
+Notation "'Sc_t'" := (fun e => is_true (is_sc lab_t e)).
+
+Notation "'b_t'" := (ThreadEvent rtid i_b).
+Notation "'a_t'" := (ThreadEvent rtid i_a).
+Notation "'mapper'" := (mapper a_t b_t).
 
 Definition prefix_closed
     (t : thread_id) :
@@ -55,7 +109,7 @@ Definition correct_op_at : Prop :=
     (
       WCore.lab_is_r (trace_nth (index a_t) tr (Afence Opln)) ∪₁
       WCore.lab_is_w (trace_nth (index a_t) tr (Afence Opln))
-    ) b_t.
+    ) a_t.
 
 Definition correct_mod_bt : Prop :=
   forall (tr : trace label)
@@ -72,10 +126,7 @@ Definition correct_mod_at : Prop :=
     )).
 
 Record correct_traces_t : Prop := {
-  prf_at_tid : tid a_t <> tid_init;
-  prf_tid : tid b_t = tid a_t;
-  prf_at_bt_neq : a_t <> b_t;
-  prf_bt_at_imm : immediate ext_sb b_t a_t;
+  prf_at_tid : rtid <> tid_init;
   prf_closed : forall t (NINIT : t <> tid_init), prefix_closed t;
   prf_cov : full_coverage;
   prf_loc : correct_loc;
@@ -96,5 +147,104 @@ Lemma simrel_xmm_step
 Proof using.
   admit.
 Admitted.
+
+Lemma corr_coh_inv
+    (WF : Wf G_t)
+    (RFC : rf_complete G_t)
+    (INIT : is_init ⊆₁ E_t)
+    (DEP : rmw_dep_t ≡ ∅₂)
+    (DATA : data_t ≡ ∅₂)
+    (CTRL : ctrl_t ≡ ∅₂)
+    (ADDR : addr_t ≡ ∅₂)
+    (CONT : contigious_actids G_t)
+    (CORR : correct_traces_t)
+    (FIN : set_finite (E_t \₁ is_init))
+    (COH : trace_coherent traces_t G_t)
+    (INITTID : E_t ∩₁ (fun e => tid e = tid_init) ⊆₁ is_init)
+    (RMWD : rmw G_t ⊆ Sc_t × Sc_t) :
+  reord_step_pred X_t a_t b_t.
+Proof using.
+  set (tr := thread_trace G_t rtid).
+  assert (NINIT : rtid <> tid_init) by apply CORR.
+  assert (EXTSB : ext_sb b_t a_t).
+  { unfold ext_sb, i_a. split; auto; lia. }
+  assert (NACQ : eq a_t ∩₁ E_t ⊆₁ set_compl Acq_t).
+  { unfolder. intros x (EQ & XIN). subst x.
+    intro FALSO. apply (prf_mod_at CORR) with tr; auto.
+    { apply event_memE; auto. }
+    unfold WCore.lab_mode, is_acq in *.
+    subst tr. rewrite thread_trace_nth'; auto. }
+  assert (NREL : eq b_t ∩₁ E_t ⊆₁ set_compl Rel_t).
+  { unfolder. intros x (EQ & XIN). subst x.
+    intro FALSO. apply (prf_mod_bt CORR) with tr; auto.
+    { apply event_memE; auto. }
+    unfold WCore.lab_mode, is_rel in *.
+    subst tr. rewrite thread_trace_nth'; auto. }
+  constructor; ins.
+  { unfolder. intros x (EQ & XIN). subst x.
+    destruct (prf_op_at CORR tr) as [ISR|ISW].
+    { apply COH, CORR. }
+    { apply event_memE; auto. }
+    { right. unfold WCore.lab_is_r, is_r in *.
+      subst tr.
+      rewrite thread_trace_nth' in ISR; auto.
+      desf. }
+    left. unfold WCore.lab_is_w, is_w in *.
+    subst tr.
+    rewrite thread_trace_nth' in ISW; auto.
+    desf. }
+  { unfolder. intros x (EQ & XIN). subst x.
+    destruct (prf_op_bt CORR tr) as [ISR|ISW].
+    { apply COH, CORR. }
+    { apply event_memE; auto. }
+    { right. unfold WCore.lab_is_r, is_r in *.
+      subst tr.
+      rewrite thread_trace_nth' in ISR; auto.
+      desf. }
+    left. unfold WCore.lab_is_w, is_w in *.
+    subst tr.
+    rewrite thread_trace_nth' in ISW; auto.
+    desf. }
+  { unfolder. intros x y ((XEQ & XIN) & SLOC & (YEQ & YIN)).
+    subst x y. apply (prf_loc CORR) with tr; auto.
+    { apply event_memE; auto. }
+    { apply event_memE; auto. }
+    unfold same_loc, loc, WCore.lab_loc in *.
+    subst tr. rewrite !thread_trace_nth'; auto. }
+  { red in CONT. destruct (CONT _ NINIT) as [N EQ].
+    assert (INA' : (E_t ∩₁ (fun e => rtid = tid e)) a_t).
+    { basic_solver. }
+    enough (INB' : (E_t ∩₁ (fun e => rtid = tid e)) b_t).
+    { apply INB'. }
+    apply EQ, thread_set_iff. apply EQ, thread_set_iff in INA'.
+    unfold i_a in INA'. lia. }
+  { unfold sb. unfolder. intros x y (((XEQ & XIN) & _) & SB & YIN).
+    apply NINA. subst x. destruct y as [yl | yt yn]; ins.
+    destruct classic with (yn = i_b + 1) as [EQ|NEQ].
+    { desf. }
+    apply ext_sb_dense with (e2 := (ThreadEvent yt yn)); auto.
+    red. desf; split; ins. unfold i_a. lia. }
+  { intros x y RMW. unfolder.
+    apply (wf_rmwE WF) in RMW.
+    unfolder in RMW. destruct RMW as (XIN & RMW & YIN).
+    apply RMWD in RMW. destruct RMW as [XSC YSC].
+    splits; auto.
+    all: intro FALSO.
+    { subst x. apply NACQ with a_t; [basic_solver|].
+      unfold is_sc, is_acq in *. desf. }
+    { subst x. apply NREL with b_t; [basic_solver|].
+      unfold is_sc, is_rel in *. desf. }
+    { subst y. apply NACQ with a_t; [basic_solver|].
+      unfold is_sc, is_acq in *. desf. }
+    subst y. apply NREL with b_t; [basic_solver|].
+    unfold is_sc, is_rel in *. desf. }
+  { unfold i_a. intro FALSO. desf. lia. }
+  { unfold sb. unfolder.
+    intros x y ((XEQ & XIN) & YEQ & YIN). subst x y.
+    splits; auto. intros c (_ & BC & CIN) (_ & CA & _).
+    unfold i_a in *. ins. desf. ins. desf. lia. }
+  unfolder. intros x y (XEQ & SB & YIN). subst x.
+  apply NINA, ext_sb_dense with (e2 := y); auto.
+Qed.
 
 End ReorderingSteps.
