src/traces/ThreadTrace.v
@@ -242,6 +242,15 @@ Proof using THREAD_EVENTS.
   now rewrite trace_elems_map, trace_elems_eq_thread_events.
 Qed.
 
+Lemma thread_trace_nth n (d : label) (LT : n < N) :
+  trace_nth n thread_trace d = lab (ThreadEvent t n).
+Proof using THREAD_EVENTS.
+  rewrite trace_nth_indep with (d' := lab (ThreadEvent t 0))
+    ; unfold thread_trace.
+  { now rewrite trace_nth_map, thread_actid_trace_nth. }
+  rewrite trace_length_map, thread_actid_trace_length; ins.
+Qed.
+
 End ThreadTrace.
 
 Definition trace_coherent traces G : Prop :=
@@ -254,6 +263,21 @@ Definition exec_trace_prefix G G' : Prop :=
 (* TODO: perhaps deserves its own module *)
 Definition contigious_actids G : Prop := forall t (NOT_INIT : t <> tid_init),
   exists N, (acts_set G) ∩₁ (fun e => t = tid e) ≡₁ thread_seq_set t N.
+
+Lemma thread_trace_nth' G e (d : label)
+    (NINIT : tid e <> tid_init)
+    (CONT : contigious_actids G)
+    (IN : acts_set G e) :
+  trace_nth (index e) (thread_trace G (tid e)) d = lab G e.
+Proof using.
+  unfold tid in *.
+  destruct e as [el | et en]; [congruence |].
+  red in CONT. destruct (CONT _ NINIT) as [N EQ].
+  rewrite thread_trace_nth with (N := N); eauto.
+  assert (IN' : (acts_set G ∩₁ (fun e => et = tid e)) (ThreadEvent et en)).
+  { basic_solver. }
+  ins. now apply EQ, thread_set_iff in IN'.
+Qed.
 
 Lemma cont_actids_sub G N t
     (EQ : (acts_set G) ∩₁ (fun e => t = tid e) ≡₁ thread_seq_set t N) :
